

AHMADU BELLO UNIVERSITY DISTANCE LEARNING CENTRE

COURSE: ALGEBRA

COURSE CODE: MATH102

**LECTURE NOTE 002: REMAINDER THEOREM AND FACTOR
THEOREM**

TUTOR: Dr. M. O. Oni

2.1 Learning Outcomes

After studying this session, I expect you to be able to:

1. State and apply the remainder theorem
2. comprehend the factor theorem and its applications

2.2 Remainder Theorem

The remainder theorem is a powerful tool for the roots of any polynomial equation.

Remainder theorem: States that if a polynomial $p(x)$ is divided by $(x - a)$ then the remainder, R is given by $R = p(a)$

Proof

Let $p(x)$ be the given polynomial in (x) ,

Let $Q(x)$ be any quotient when $p(x)$ is divided by $(x - a)$ and let R be the remainder.

Thus $\frac{p(x)}{(x-a)} = Q(x) + \frac{R}{x-a}$ where R is the remainder

$$p(x) = Q(x)(x - a) + R$$

Putting $x = a$, then we have:

$$p(a) = Q(a)(a - a) + R$$

$$p(a) = R \text{ (Q.E.D)}$$

Example 2.1: Find the remainder when $4x^3 - 2x^2 + 4x - 1$ is divided by

(i) $(x + 2)$

(ii) $(x - 4)$

(iii) $(x + 1)$

(iv) x

Solution

Let $y(x) = 4x^3 - 2x^2 + 4x - 1$. By remainder theorem, when a polynomial is divided by a factor, the remainder is $y(a)$.

(i) Comparing $x - a$ with $x + 2$

Implies $a = -2$,

Hence the remainder is

$$\begin{aligned} y(-2) &= 4(-2)^3 - 2(-2)^2 + 4(-2) - 1 \\ &= -32 - 8 - 8 - 1 \\ &= -49 \end{aligned}$$

So that the remainder when $4x^3 - 2x^2 + 4x - 1$ is divided by $(x + 2)$ is:

$$y(-2) = -49$$

(ii) Comparing $x - a$ with $x - 4$

Implies $a = 4$,

Hence the remainder is

$$\begin{aligned} y(4) &= 4(4)^3 - 2(4)^2 + 4(4) - 1 \\ &= 256 - 32 + 16 - 1 \end{aligned}$$

So that the remainder when $4x^3 - 2x^2 + 4x - 1$ is divided by $(x - 4)$ is:

$$y(4) = 239$$

(iii) Comparing $x - a$ with $x + 1$

Implies $a = -1$,

Hence the remainder is

$$\begin{aligned} y(-1) &= 4(-1)^3 - 2(-1)^2 + 4(-1) - 1 \\ &= -4 - 2 - 4 - 1 \end{aligned}$$

So that the remainder when $4x^3 - 2x^2 + 4x - 1$ is divided by $(x + 1)$ is:

$$y(-1) = -11$$

(iv) Comparing $x - a$ with x

Implies $a = 0$,

Hence the remainder is

$$\begin{aligned} y(0) &= 4(0)^3 - 2(0)^2 + 4(0) - 1 \\ &= -1 \end{aligned}$$

So that the remainder when $4x^3 - 2x^2 + 4x - 1$ is divided by (x) is:

$$y(0) = -1$$

Example 2.2: Find the remainder when $3x^2 - 4x + 2$ is divided by

(a) $(x - 2)$

(b) $(x + 1)$

Solution

(a) Let $p(x) = 3x^2 - 4x + 2$, the remainder when $p(x)$ is divided by $(x - 2)$ is

$$p(2)$$

$$p(2) = 3(2)^2 - 4(2) + 2$$

$$p(2) = 12 - 8 + 2$$

$$\text{So that } p(2) = 6$$

Hence the remainder when $3x^2 - 4x + 2$ is divided by $(x - 2)$ is 6

(b) Let $p(x) = 3x^2 - 4x + 2$, the remainder when $p(x)$ is divided by $(x + 1)$ is $p(-1)$

$$p(-1) = 3(-1)^2 - 4(-1) + 2$$

$$p(-1) = 3 + 4 + 2$$

$$\text{So that } p(-1) = 9$$

Hence the remainder when $3x^2 - 4x + 2$ is divided by $(x + 1)$ is 9

2.3 Factor Theorem

Factor Theorem: if $p(x)$ is a polynomial in x and remainder $R = p(a) = 0$, when divided by $(x - a)$, then $(x - a)$ is a factor of $p(x)$.

In fact, if $p(a) = 0$, then a is a root of the polynomial equation $p(x) = 0$.

Proof:

Let $p(x)$ be the given polynomial in (x) ,

Let $Q(x)$ be any quotient when $p(x)$ is divided by $(x - a)$ and let R be the remainder.

$$\text{Thus } \frac{p(x)}{(x-a)} = Q(x) + \frac{R}{x-a} \quad \text{where } R \text{ is the remainder}$$

If $R = 0$, then

$$p(x) = Q(x)(x - a) + 0$$

Putting $x = a$, then we have

$$p(a) = Q(a)(a - a)$$

$$p(a) = 0$$

Example 2.3: Determine whether (i) $(x - 1)$ and (ii) $(x + 1)$ is a factor of the cubic equation $x^3 - 2x^2 - 5x + 6 = 0$.

Solution

Let $p(x) = x^3 - 2x^2 - 5x + 6$, by factor theorem, if $(x - a)$ is factor of the polynomial $p(x)$, then $p(a) = 0$.

(i) So that $a = 1$, hence, $p(1)$

$$p(1) = 1^3 - 2(1)^2 - 5(1) + 6$$

$$p(1) = 1 - 2 - 5 + 6$$

$$p(1) = 0,$$

Hence $(x - 1)$ is a factor of the equation $x^3 - 2x^2 - 5x + 6 = 0$.

(ii) Also, $a = -1$, hence, $p(-1)$

$$p(-1) = (-1)^3 - 2(-1)^2 - 5(-1) + 6$$

$$p(-1) = -1 - 2 + 5 + 6$$

$$p(-1) = 8,$$

Since $p(-1) \neq 0$, hence $(x + 1)$ is not a factor of the equation $x^3 - 2x^2 - 5x + 6 = 0$.

Example 2.4: Solve $x^4 - 15x^2 - 10x + 24 = 0$

Solution

Using factor theorem,

$$\text{Let } p(x) = x^4 - 15x^2 - 10x + 24$$

By inspection, $p(1) = 0$ which means $(x - 1)$ is a factor,

Next, $p(2) \neq 0$, which means $(x - 2)$ is not a factor

By further inspection, $p(-2) = 0$ which means $(x + 2)$ is a factor

Similarly, $p(-3) = 0$ which means $(x + 3)$ is a factor

And $p(4) = 0$ which means $(x - 4)$ is a factor

$$\text{So that } x^4 - 15x^2 - 10x + 24 = (x - 1)(x + 2)(x + 3)(x - 4)$$

So that the roots of the quartic equation $x^4 - 15x^2 - 10x + 24 = 0$ are $x = 1, -2, -3, 4$

Example 2.4: Factorize $x^4 - 5x^2 + 4$, and hence find the roots of $x^4 - 5x^2 + 4 = 0$

Solution

$$\text{Let } p(x) = x^4 - 5x^2 + 4, \text{ By inspection } p(-1) = p(1) = p(2) = p(-2) = 0$$

Hence $(x - 1)(x + 1)(x - 2)(x + 2)$ are factors

$$\text{So that } x^4 - 5x^2 + 4 = (x - 1)(x + 1)(x - 2)(x + 2)$$

And the roots of $x^4 - 5x^2 + 4 = 0$ are $x = -1, 1, -2, 2$

2.4 Principle of undetermined coefficient

If two polynomial expression in x are equal for all values of x , we can equate the like powers of x . i.e If

$a_n x^n + a_{n-1} x^{n-1} + a_{n-2} x^{n-2} + \dots + a_1 x + a_0 = b_{n-1} x^{n-1} + b_{n-2} x^{n-2} + \dots + b_1 x + b_0$. Then $a_n = 0$, $a_{n-1} = b_{n-1}$, \dots , $a_1 = b_1$, $a_0 = b_0$. The principle stated is called the principle of undetermined coefficient e.g

Example 2.6: Determine the values of s , t and u .If

$$2x^2 + 3x + 8 = s(x + 1)(x - 2) + t(x + 3) + u,$$

Solution

By the principle of undetermined coefficient,

$$2x^2 + 3x + 8 = s(x^2 - x - 2) + t(x + 3) + u,$$

$$\text{Implies, } 2x^2 + 3x + 8 = sx^2 + x(t - s) + 3t - 2s + u,$$

By principle of undetermined coefficient,

$$s = 2,$$

$$\text{Then } (t - s) = 3 \text{ which implies } t = 5$$

$$\text{and } 3t - 2s + u = 8,$$

$$\text{which makes } u = -3$$

In-text Question 1: If $p(a) = -1$ then $(x - a)$ is a factor of the polynomial (TRUE/ FALSE)

2. If $p(a) = 0$ then $(x - a)$ is a factor of the polynomial (TRUE/ FALSE)

Exercise

1. Determine the remainder when $x^3 - 6x^2 + x - 5$ is divided by

(a) $(x + 2)$ (b) $(x - 3)$

2. Solve the cubic equation $x^3 - 2x^2 - 5x + 6 = 0$ by using the factor theorem

3. Find the remainder when $2x^5 - 2x^3 + 4x^2 - 12x + 3$ is divided by

(i) $(x - 2)$ (ii) $(x - 4)$ (iii) $(x - 1/2)$ (iv) $(x - 10)$

4. If $(x - 1)$ and $(x + 2)$ are factors of $p(x) = x^4 + bx^3 + 4x^2 + cx - 4$, find the value of b and c . show that with these value of b and c , $(x + 1)$ is also a factor of $p(x)$ and find the fourth factor.

5. Solve the equation $x^3 - 2x^2 - x + 2 = 0$.

6. Determine the value of 'a' if $(x + 2)$ is a factor of $x^3 - ax^2 + 14x + 8 = 0$.

7. Determine the remainder when $x^3 - 6x^2 + x - 5$ is divided by

(a) $(x + 2)$ (b) $(x - 3)$

8. Solve the cubic equation $x^3 - 2x^2 - 5x + 6 = 0$ by using the factor theorem

9. Find the remainder when $2x^5 - 2x^3 + 4x^2 - 12x + 3$ is divided by

(i) $(x - 2)$ (ii) $(x - 4)$ (iii) $(x - 1/2)$ (iv) $(x - 10)$

10. Solve (i) $x^4 - 10x^3 + 35x^2 - 50x + 24 = 0$

(ii) $x^4 - 41x^2 + 400 = 0$

2.5 Conclusion/Summary

In this section, the remainder theorem as well as the factor theorem have been presented. We have established that for any given polynomial $p(x)$, the remainder when divided by $(x - a)$ is $p(a)$. In addition, we showed that if the remainder is zero, i.e $p(a) = 0$, then $(x - a)$ is a factor of the polynomial $p(x)$. In fact, $x = a$ is a root of the polynomial $p(x)$.

References/Further Readings

“Course code: Course Title, National Open University of Nigeria, 2014 at <http://www.nou.edu.ng/index.htm#>

John Bird (2006), Higher Engineering Mathematics, 5th Edition, Linacre House, Jordan Hill, Oxford OX2 8DP 30 Corporate Drive, Suite 400, Burlington, MA01803, USA.

Wikipedia contributors. (2018, November 17). Cubic function.
https://en.wikipedia.org/w/index.php?title=Cubic_function&oldid=869250796

Wikipedia contributors. (2018, November 6). Quartic function.
https://en.wikipedia.org/w/index.php?title=Quartic_function&oldid=867550556

MATH102 LECTURE NOTE 002, Dr. M. O. Oni